Some small changes to the examples

tutorial/utp_csp_mini_mondex.thy
@@ -16,7 +16,7 @@ text {* In the paper money is represented as a nat, here we use an int so that w
   of modelling negative balances. This also eases proof as integers form an algebraic ring. *}
   
 alphabet st_mdx =
-  valueseq :: "money list" -- {* Index record of each card's balance *}
+  accts :: "money list" -- {* Index record of each card's balance *}
   
 datatype ch_mdx = 
   pay "index \<times> index \<times> money" | -- {* Request a payment between two cards *}
@@ -39,9 +39,9 @@ definition Pay :: "index \<Rightarrow> index \<Rightarrow> money \<Rightarrow> a
 "Pay i j n = 
   pay.(\<guillemotleft>i\<guillemotright>).(\<guillemotleft>j\<guillemotright>).(\<guillemotleft>n\<guillemotright>) \<^bold>\<rightarrow> 
     ((reject.(\<guillemotleft>i\<guillemotright>) \<^bold>\<rightarrow> Skip) 
-      \<triangleleft> \<guillemotleft>i\<guillemotright> =\<^sub>u \<guillemotleft>j\<guillemotright> \<or> \<guillemotleft>n\<guillemotright> \<le>\<^sub>u 0 \<or> \<guillemotleft>n\<guillemotright> >\<^sub>u &valueseq\<lparr>\<guillemotleft>i\<guillemotright>\<rparr>\<^sub>u \<triangleright>\<^sub>R 
-    ({valueseq[\<guillemotleft>i\<guillemotright>]} :=\<^sub>C (&valueseq\<lparr>\<guillemotleft>i\<guillemotright>\<rparr>\<^sub>u - \<guillemotleft>n\<guillemotright>) ;;
-     {valueseq[\<guillemotleft>j\<guillemotright>]} :=\<^sub>C (&valueseq\<lparr>\<guillemotleft>j\<guillemotright>\<rparr>\<^sub>u + \<guillemotleft>n\<guillemotright>) ;;
+      \<triangleleft> \<guillemotleft>i\<guillemotright> =\<^sub>u \<guillemotleft>j\<guillemotright> \<or> \<guillemotleft>n\<guillemotright> \<le>\<^sub>u 0 \<or> \<guillemotleft>n\<guillemotright> >\<^sub>u &accts\<lparr>\<guillemotleft>i\<guillemotright>\<rparr>\<^sub>u \<triangleright>\<^sub>R 
+    ({accts[\<guillemotleft>i\<guillemotright>]} :=\<^sub>C (&accts\<lparr>\<guillemotleft>i\<guillemotright>\<rparr>\<^sub>u - \<guillemotleft>n\<guillemotright>) ;;
+     {accts[\<guillemotleft>j\<guillemotright>]} :=\<^sub>C (&accts\<lparr>\<guillemotleft>j\<guillemotright>\<rparr>\<^sub>u + \<guillemotleft>n\<guillemotright>) ;;
      accept.(\<guillemotleft>i\<guillemotright>) \<^bold>\<rightarrow> Skip))"
     
 definition PaySet :: "index \<Rightarrow> (index \<times> index \<times> money) set" where
@@ -60,7 +60,7 @@ text {* The Mondex action is a sample setup. It requires creates $cardNum$ cards
   present. *}
 
 definition Mondex :: "index \<Rightarrow> action_mdx" where
-"Mondex(cardNum) = (valueseq :=\<^sub>C \<guillemotleft>replicate cardNum 100\<guillemotright> ;; Cycle(cardNum))"
+"Mondex(cardNum) = (accts :=\<^sub>C \<guillemotleft>replicate cardNum 100\<guillemotright> ;; Cycle(cardNum))"
 
 subsection {* Pre/peri/post calculations *}
 
@@ -83,7 +83,7 @@ text {* The precondition of pay requires that, under the assumption that a payme
   
 lemma preR_Pay [rdes]:
   "pre\<^sub>R(Pay i j n) = 
-    ($tr ^\<^sub>u \<langle>(pay\<cdot>\<guillemotleft>(i, j, n)\<guillemotright>)\<^sub>u\<rangle> \<le>\<^sub>u $tr\<acute> \<and> \<guillemotleft>i\<guillemotright> \<noteq>\<^sub>u \<guillemotleft>j\<guillemotright> \<and> 0 <\<^sub>u \<guillemotleft>n\<guillemotright> \<and> \<guillemotleft>n\<guillemotright> \<le>\<^sub>u $st:valueseq\<lparr>\<guillemotleft>i\<guillemotright>\<rparr>\<^sub>u \<Rightarrow> {\<guillemotleft>i\<guillemotright>,\<guillemotleft>j\<guillemotright>}\<^sub>u \<subseteq>\<^sub>u dom\<^sub>u($st:valueseq))"
+    ($tr ^\<^sub>u \<langle>(pay\<cdot>\<guillemotleft>(i, j, n)\<guillemotright>)\<^sub>u\<rangle> \<le>\<^sub>u $tr\<acute> \<and> \<guillemotleft>i\<guillemotright> \<noteq>\<^sub>u \<guillemotleft>j\<guillemotright> \<and> 0 <\<^sub>u \<guillemotleft>n\<guillemotright> \<and> \<guillemotleft>n\<guillemotright> \<le>\<^sub>u $st:accts\<lparr>\<guillemotleft>i\<guillemotright>\<rparr>\<^sub>u \<Rightarrow> {\<guillemotleft>i\<guillemotright>,\<guillemotleft>j\<guillemotright>}\<^sub>u \<subseteq>\<^sub>u dom\<^sub>u($st:accts))"
   apply (simp add: Pay_def closure rdes unrest alpha usubst wp)
   apply (rel_auto) using dual_order.trans by blast
  
@@ -94,8 +94,8 @@ text {* The pericondition has three cases: (1) nothing has happened and we are n
 lemma periR_Pay [rdes]:
   "peri\<^sub>R(Pay i j n) = 
     (pre\<^sub>R(Pay i j n) \<Rightarrow> $tr\<acute> =\<^sub>u $tr \<and> (pay\<cdot>\<guillemotleft>(i, j, n)\<guillemotright>)\<^sub>u \<notin>\<^sub>u $ref\<acute>
-                     \<or> $tr\<acute> =\<^sub>u $tr ^\<^sub>u \<langle>(pay\<cdot>\<guillemotleft>(i, j, n)\<guillemotright>)\<^sub>u\<rangle> \<and> (\<guillemotleft>i\<guillemotright> =\<^sub>u \<guillemotleft>j\<guillemotright> \<or> \<guillemotleft>n\<guillemotright> \<le>\<^sub>u 0 \<or> \<guillemotleft>n\<guillemotright> >\<^sub>u $st:valueseq\<lparr>\<guillemotleft>i\<guillemotright>\<rparr>\<^sub>u) \<and> (reject\<cdot>\<guillemotleft>i\<guillemotright>)\<^sub>u \<notin>\<^sub>u $ref\<acute>
-                     \<or> $tr\<acute> =\<^sub>u $tr ^\<^sub>u \<langle>(pay\<cdot>\<guillemotleft>(i, j, n)\<guillemotright>)\<^sub>u\<rangle> \<and> \<guillemotleft>i\<guillemotright> \<noteq>\<^sub>u \<guillemotleft>j\<guillemotright> \<and> 0 <\<^sub>u \<guillemotleft>n\<guillemotright> \<and> \<guillemotleft>n\<guillemotright> \<le>\<^sub>u $st:valueseq\<lparr>\<guillemotleft>i\<guillemotright>\<rparr>\<^sub>u \<and> (accept\<cdot>\<guillemotleft>i\<guillemotright>)\<^sub>u \<notin>\<^sub>u $ref\<acute>)"
+                     \<or> $tr\<acute> =\<^sub>u $tr ^\<^sub>u \<langle>(pay\<cdot>\<guillemotleft>(i, j, n)\<guillemotright>)\<^sub>u\<rangle> \<and> (\<guillemotleft>i\<guillemotright> =\<^sub>u \<guillemotleft>j\<guillemotright> \<or> \<guillemotleft>n\<guillemotright> \<le>\<^sub>u 0 \<or> \<guillemotleft>n\<guillemotright> >\<^sub>u $st:accts\<lparr>\<guillemotleft>i\<guillemotright>\<rparr>\<^sub>u) \<and> (reject\<cdot>\<guillemotleft>i\<guillemotright>)\<^sub>u \<notin>\<^sub>u $ref\<acute>
+                     \<or> $tr\<acute> =\<^sub>u $tr ^\<^sub>u \<langle>(pay\<cdot>\<guillemotleft>(i, j, n)\<guillemotright>)\<^sub>u\<rangle> \<and> \<guillemotleft>i\<guillemotright> \<noteq>\<^sub>u \<guillemotleft>j\<guillemotright> \<and> 0 <\<^sub>u \<guillemotleft>n\<guillemotright> \<and> \<guillemotleft>n\<guillemotright> \<le>\<^sub>u $st:accts\<lparr>\<guillemotleft>i\<guillemotright>\<rparr>\<^sub>u \<and> (accept\<cdot>\<guillemotleft>i\<guillemotright>)\<^sub>u \<notin>\<^sub>u $ref\<acute>)"
   by (simp add: Pay_def closure rdes unrest alpha usubst wp, rel_auto)
     
 text {* The postcondition has two options. Firstly, the amount was wrong, and so the trace was extended
@@ -104,9 +104,9 @@ text {* The postcondition has two options. Firstly, the amount was wrong, and so
     
 lemma postR_Pay [rdes]:
   "post\<^sub>R(Pay i j n) = 
-    (pre\<^sub>R(Pay i j n) \<Rightarrow> $tr\<acute> =\<^sub>u $tr ^\<^sub>u \<langle>(pay\<cdot>\<guillemotleft>(i, j, n)\<guillemotright>)\<^sub>u,(reject\<cdot>\<guillemotleft>i\<guillemotright>)\<^sub>u\<rangle> \<and> (\<guillemotleft>i\<guillemotright> =\<^sub>u \<guillemotleft>j\<guillemotright> \<or> \<guillemotleft>n\<guillemotright> \<le>\<^sub>u 0 \<or> \<guillemotleft>n\<guillemotright> >\<^sub>u $st:valueseq\<lparr>\<guillemotleft>i\<guillemotright>\<rparr>\<^sub>u) \<and> $st\<acute> =\<^sub>u $st
-                     \<or> $tr\<acute> =\<^sub>u $tr ^\<^sub>u \<langle>(pay\<cdot>\<guillemotleft>(i, j, n)\<guillemotright>)\<^sub>u,(accept\<cdot>\<guillemotleft>i\<guillemotright>)\<^sub>u\<rangle> \<and> \<guillemotleft>i\<guillemotright> \<noteq>\<^sub>u \<guillemotleft>j\<guillemotright> \<and> 0 <\<^sub>u \<guillemotleft>n\<guillemotright> \<and> \<guillemotleft>n\<guillemotright> \<le>\<^sub>u $st:valueseq\<lparr>\<guillemotleft>i\<guillemotright>\<rparr>\<^sub>u 
-                       \<and> \<lceil>valueseq := &valueseq(\<guillemotleft>i\<guillemotright> \<mapsto> &valueseq\<lparr>\<guillemotleft>i\<guillemotright>\<rparr>\<^sub>u - \<guillemotleft>n\<guillemotright>, \<guillemotleft>j\<guillemotright> \<mapsto> &valueseq\<lparr>\<guillemotleft>j\<guillemotright>\<rparr>\<^sub>u + \<guillemotleft>n\<guillemotright>)\<^sub>u\<rceil>\<^sub>S)"
+    (pre\<^sub>R(Pay i j n) \<Rightarrow> $tr\<acute> =\<^sub>u $tr ^\<^sub>u \<langle>(pay\<cdot>\<guillemotleft>(i, j, n)\<guillemotright>)\<^sub>u,(reject\<cdot>\<guillemotleft>i\<guillemotright>)\<^sub>u\<rangle> \<and> (\<guillemotleft>i\<guillemotright> =\<^sub>u \<guillemotleft>j\<guillemotright> \<or> \<guillemotleft>n\<guillemotright> \<le>\<^sub>u 0 \<or> \<guillemotleft>n\<guillemotright> >\<^sub>u $st:accts\<lparr>\<guillemotleft>i\<guillemotright>\<rparr>\<^sub>u) \<and> $st\<acute> =\<^sub>u $st
+                     \<or> $tr\<acute> =\<^sub>u $tr ^\<^sub>u \<langle>(pay\<cdot>\<guillemotleft>(i, j, n)\<guillemotright>)\<^sub>u,(accept\<cdot>\<guillemotleft>i\<guillemotright>)\<^sub>u\<rangle> \<and> \<guillemotleft>i\<guillemotright> \<noteq>\<^sub>u \<guillemotleft>j\<guillemotright> \<and> 0 <\<^sub>u \<guillemotleft>n\<guillemotright> \<and> \<guillemotleft>n\<guillemotright> \<le>\<^sub>u $st:accts\<lparr>\<guillemotleft>i\<guillemotright>\<rparr>\<^sub>u 
+                       \<and> \<lceil>accts := &accts(\<guillemotleft>i\<guillemotright> \<mapsto> &accts\<lparr>\<guillemotleft>i\<guillemotright>\<rparr>\<^sub>u - \<guillemotleft>n\<guillemotright>, \<guillemotleft>j\<guillemotright> \<mapsto> &accts\<lparr>\<guillemotleft>j\<guillemotright>\<rparr>\<^sub>u + \<guillemotleft>n\<guillemotright>)\<^sub>u\<rceil>\<^sub>S)"
   by (simp add: Pay_def closure rdes unrest alpha usubst wp, rel_simp, safe, simp_all, blast+)    
             
 lemma Pay_wf [closure]:
@@ -130,7 +130,7 @@ lemma AllPay_Productive [closure]:
     
 lemma preR_AllPay [rdes]:
   "cardNum \<ge> 2 \<Longrightarrow> pre\<^sub>R(AllPay cardNum) = 
-    (\<Squnion> (i, j, n) \<in> PaySet cardNum \<bullet> $tr\<acute> \<ge>\<^sub>u $tr ^\<^sub>u \<langle>(pay\<cdot>\<guillemotleft>(i, j, n)\<guillemotright>)\<^sub>u\<rangle> \<and> \<guillemotleft>i\<guillemotright> \<noteq>\<^sub>u \<guillemotleft>j\<guillemotright> \<and> \<guillemotleft>n\<guillemotright> >\<^sub>u 0 \<and> $st:valueseq\<lparr>\<guillemotleft>i\<guillemotright>\<rparr>\<^sub>u \<ge>\<^sub>u \<guillemotleft>n\<guillemotright> \<Rightarrow> {\<guillemotleft>i\<guillemotright>, \<guillemotleft>j\<guillemotright>}\<^sub>u \<subseteq>\<^sub>u dom\<^sub>u($st:valueseq))"
+    (\<Squnion> (i, j, n) \<in> PaySet cardNum \<bullet> $tr\<acute> \<ge>\<^sub>u $tr ^\<^sub>u \<langle>(pay\<cdot>\<guillemotleft>(i, j, n)\<guillemotright>)\<^sub>u\<rangle> \<and> \<guillemotleft>i\<guillemotright> \<noteq>\<^sub>u \<guillemotleft>j\<guillemotright> \<and> \<guillemotleft>n\<guillemotright> >\<^sub>u 0 \<and> $st:accts\<lparr>\<guillemotleft>i\<guillemotright>\<rparr>\<^sub>u \<ge>\<^sub>u \<guillemotleft>n\<guillemotright> \<Rightarrow> {\<guillemotleft>i\<guillemotright>, \<guillemotleft>j\<guillemotright>}\<^sub>u \<subseteq>\<^sub>u dom\<^sub>u($st:accts))"
   by (simp add: AllPay_def rdes closure)    
     
 subsection {* Verification *}
@@ -149,7 +149,7 @@ text {* We perform verification by writing contracts that specify desired behavi
   
 theorem money_constant:
   assumes "i < cardNum" "j < cardNum" "i \<noteq> j"
-  shows "[#\<^sub>u(&valueseq) =\<^sub>u \<guillemotleft>cardNum\<guillemotright> \<turnstile> true | sum\<^sub>u($valueseq) =\<^sub>u sum\<^sub>u($valueseq\<acute>)]\<^sub>C \<sqsubseteq> Pay i j n"
+  shows "[#\<^sub>u(&accts) =\<^sub>u \<guillemotleft>cardNum\<guillemotright> \<turnstile> true | sum\<^sub>u($accts) =\<^sub>u sum\<^sub>u($accts\<acute>)]\<^sub>C \<sqsubseteq> Pay i j n"
 -- {* We first apply the reactive design contract introduction law and discharge well-formedness of Pay *}
 proof (rule CRD_contract_refine, simp add: closure)
 
@@ -159,12 +159,12 @@ proof (rule CRD_contract_refine, simp add: closure)
     input and the money amount constraints. We discharge by first calculating the precondition, 
     as done above, and then using the relational calculus tactic. *}
 
-  from assms show "`\<lceil>#\<^sub>u(&valueseq) =\<^sub>u \<guillemotleft>cardNum\<guillemotright>\<rceil>\<^sub>S\<^sub>< \<Rightarrow> pre\<^sub>R (Pay i j n)`"
+  from assms show "`\<lceil>#\<^sub>u(&accts) =\<^sub>u \<guillemotleft>cardNum\<guillemotright>\<rceil>\<^sub>S\<^sub>< \<Rightarrow> pre\<^sub>R (Pay i j n)`"
     by (rdes_calc, rel_auto)
 
   -- {* The second is trivial as we don't care about intermediate states. *}
       
-  show "`\<lceil>#\<^sub>u(&valueseq) =\<^sub>u \<guillemotleft>cardNum\<guillemotright>\<rceil>\<^sub>S\<^sub>< \<and> peri\<^sub>R (Pay i j n) \<Rightarrow> \<lceil>true\<rceil>\<^sub>S\<^sub><\<lbrakk>x\<rightarrow>tt\<rbrakk>\<lbrakk>r\<rightarrow>$ref\<acute>\<rbrakk>`"
+  show "`\<lceil>#\<^sub>u(&accts) =\<^sub>u \<guillemotleft>cardNum\<guillemotright>\<rceil>\<^sub>S\<^sub>< \<and> peri\<^sub>R (Pay i j n) \<Rightarrow> \<lceil>true\<rceil>\<^sub>S\<^sub><\<lbrakk>x\<rightarrow>tt\<rbrakk>\<lbrakk>r\<rightarrow>$ref\<acute>\<rbrakk>`"
     by rel_auto
 
   -- {* The third requires that we show that the postcondition implies that the total amount remains
@@ -173,7 +173,7 @@ proof (rule CRD_contract_refine, simp add: closure)
     be retrieved by sledgehammer. However, we actually had to prove that property first and add it to our library. *}
       
   from assms
-  show " `\<lceil>#\<^sub>u(&valueseq) =\<^sub>u \<guillemotleft>cardNum\<guillemotright>\<rceil>\<^sub>S\<^sub>< \<and> post\<^sub>R (Pay i j n) \<Rightarrow> \<lceil>sum\<^sub>u($valueseq) =\<^sub>u sum\<^sub>u($valueseq\<acute>)\<rceil>\<^sub>S\<lbrakk>x\<rightarrow>tt\<rbrakk>`"
+  show " `\<lceil>#\<^sub>u(&accts) =\<^sub>u \<guillemotleft>cardNum\<guillemotright>\<rceil>\<^sub>S\<^sub>< \<and> post\<^sub>R (Pay i j n) \<Rightarrow> \<lceil>sum\<^sub>u($accts) =\<^sub>u sum\<^sub>u($accts\<acute>)\<rceil>\<^sub>S\<lbrakk>x\<rightarrow>tt\<rbrakk>`"
     by (rdes_calc, rel_auto, simp add: listsum_update)
 qed
 
@@ -182,7 +182,7 @@ text {* The next property is that no card value can go below 0, assuming it was 
   
 theorem no_overdrafts:
   assumes "i < cardNum" "j < cardNum" "i \<noteq> j"
-  shows "[#\<^sub>u(&valueseq) =\<^sub>u \<guillemotleft>cardNum\<guillemotright> \<turnstile> true | (\<^bold>\<forall> k \<bullet> \<guillemotleft>k\<guillemotright> <\<^sub>u \<guillemotleft>cardNum\<guillemotright> \<and> $valueseq\<lparr>\<guillemotleft>k\<guillemotright>\<rparr>\<^sub>u \<ge>\<^sub>u 0 \<Rightarrow> $valueseq\<acute>\<lparr>\<guillemotleft>k\<guillemotright>\<rparr>\<^sub>u \<ge>\<^sub>u 0)]\<^sub>C \<sqsubseteq> Pay i j n"
+  shows "[#\<^sub>u(&accts) =\<^sub>u \<guillemotleft>cardNum\<guillemotright> \<turnstile> true | (\<^bold>\<forall> k \<bullet> \<guillemotleft>k\<guillemotright> <\<^sub>u \<guillemotleft>cardNum\<guillemotright> \<and> $accts\<lparr>\<guillemotleft>k\<guillemotright>\<rparr>\<^sub>u \<ge>\<^sub>u 0 \<Rightarrow> $accts\<acute>\<lparr>\<guillemotleft>k\<guillemotright>\<rparr>\<^sub>u \<ge>\<^sub>u 0)]\<^sub>C \<sqsubseteq> Pay i j n"
   apply (rule CRD_contract_refine)
   apply (simp add: Pay_def closure)
   apply (simp add: rdes)
@@ -200,8 +200,8 @@ text {* The next property shows liveness of transfers. If a payment is accepted,
   
 theorem transfer_live:
   assumes "i < cardNum" "j < cardNum" "i \<noteq> j" "n > 0"
-  shows "[#\<^sub>u(&valueseq) =\<^sub>u \<guillemotleft>cardNum\<guillemotright> 
-         \<turnstile> \<guillemotleft>trace\<guillemotright> \<noteq>\<^sub>u \<langle>\<rangle> \<and> last\<^sub>u(\<guillemotleft>trace\<guillemotright>) =\<^sub>u (pay\<cdot>(\<guillemotleft>(i,j,k)\<guillemotright>))\<^sub>u \<and> \<guillemotleft>n\<guillemotright> \<le>\<^sub>u &valueseq\<lparr>\<guillemotleft>i\<guillemotright>\<rparr>\<^sub>u \<Rightarrow> (accept\<cdot>(\<guillemotleft>(i)\<guillemotright>))\<^sub>u \<notin>\<^sub>u \<guillemotleft>refs\<guillemotright>
+  shows "[#\<^sub>u(&accts) =\<^sub>u \<guillemotleft>cardNum\<guillemotright> 
+         \<turnstile> \<guillemotleft>trace\<guillemotright> \<noteq>\<^sub>u \<langle>\<rangle> \<and> last\<^sub>u(\<guillemotleft>trace\<guillemotright>) =\<^sub>u (pay\<cdot>(\<guillemotleft>(i,j,k)\<guillemotright>))\<^sub>u \<and> \<guillemotleft>n\<guillemotright> \<le>\<^sub>u &accts\<lparr>\<guillemotleft>i\<guillemotright>\<rparr>\<^sub>u \<Rightarrow> (accept\<cdot>(\<guillemotleft>(i)\<guillemotright>))\<^sub>u \<notin>\<^sub>u \<guillemotleft>refs\<guillemotright>
          | true]\<^sub>C \<sqsubseteq> Pay i j n"
   apply (rule_tac CRD_contract_refine)
   apply (simp add: Pay_def closure)
